LeanMqtt.lean
@@ -2,3 +2,4 @@
 -- Import modules here that should be built as part of the library.
 import LeanMqtt.Defs.Packets.Packet
 import LeanMqtt.Serialization.Packets.Packet
+import LeanMqtt.Proofs.Packets.Packet
